tests/eval/certirocq_eval_issue.v
@@ -37,12 +37,12 @@ Definition test : nat := (nth l (3000; nth_l)).
 (* Time Eval vm_compute in test. *)
 (* 30 seconds, includes cost of building the intermediate n < length proofs  *)
 (* Stack overflowing when replacing 4000 with 45000 for example? *)
-(* CertiRocq Eval -debug -time test. *)
+(* CertiRocq Eval --debug --time test. *)
 Definition largenat := 45000.
 (* Stack overflowing? *)
 
 Definition llength := length l.
-CertiRocq Eval -debug -time llength.
+CertiRocq Eval --debug --time llength.
 
 Time Eval vm_compute in llength.
 Time Eval native_compute in llength.
